MercVerified/Code/FunsExternal.lean
@@ -1,1 +1,16 @@
 import MercVerified.Code.FunsExternal_Template
+
+open Aeneas Aeneas.Std Result
+
+@[trait_default]
+def core.cmp.Eq.assert_fields_are_eq.default
+  {Self : Type} (_ : core.cmp.Eq Self) (_ : Self) : Result Unit :=
+  .ok ()
+
+def
+  merc_utilities.tagged_index.TagIndex.Insts.CoreCmpEq.assert_fields_are_eq
+  {T : Type} (Tag : Type) (_corecmpEqInst : core.cmp.Eq T)
+  (_self : merc_utilities.tagged_index.TagIndex T Tag) :
+  Result Unit
+  := do
+  ok ()
